Semantics/IRStepThms.thy
@@ -91,31 +91,31 @@ proof (induction rule: "step.induct")
   have notif: "\<not>(is_IfNode (kind g nid))"
     by (metis is_IfNode_def SequentialNode.hyps(1) is_sequential_node.simps(22))
   have notend: "\<not>(is_AbstractEndNode (kind g nid))"
-    by (metis is_AbstractEndNode.simps SequentialNode.hyps(1) is_sequential_node.simps(18,35)
+    by (metis is_AbstractEndNode.simps SequentialNode.hyps(1) is_sequential_node.simps(18,36)
         is_EndNode.elims(2) is_LoopEndNode_def)
   have notnew: "\<not>(is_NewInstanceNode (kind g nid))"
-    by (metis is_NewInstanceNode_def SequentialNode.hyps(1) is_sequential_node.simps(41))
+    by (metis is_NewInstanceNode_def SequentialNode.hyps(1) is_sequential_node.simps(42))
   have notload: "\<not>(is_LoadFieldNode (kind g nid))"
     by (metis is_LoadFieldNode_def SequentialNode.hyps(1) is_sequential_node.simps(33))
   have notstore: "\<not>(is_StoreFieldNode (kind g nid))"
-    by (metis is_StoreFieldNode_def SequentialNode.hyps(1) is_sequential_node.simps(53))
+    by (metis is_StoreFieldNode_def SequentialNode.hyps(1) is_sequential_node.simps(54))
   have notdivrem:  "\<not>(is_IntegerDivRemNode (kind g nid))"
-    by (metis is_IntegerDivRemNode.simps SequentialNode.hyps(1) is_sequential_node.simps(51,52)
+    by (metis is_IntegerDivRemNode.simps SequentialNode.hyps(1) is_sequential_node.simps(52,53)
         is_SignedDivNode_def is_SignedRemNode_def)
   from notif notend notnew notload notstore notdivrem
   show ?case
-    by (smt (verit) SequentialNode Pair_inject IRNode.disc(870,1614,3102) IRNode.discI(38)
-        step.cases is_sequential_node.simps(12,14,20,40,51,52))
+    by (smt (verit) SequentialNode Pair_inject IRNode.disc(898,1666,3266) IRNode.discI(39)
+        step.cases is_sequential_node.simps(12,14,20,34,41,52,53,55))
 next
   case (FixedGuardNode nid cond before "next" condE m p val h)
   have notseq: "\<not>(is_sequential_node (kind g nid))"
     using is_sequential_node.simps by (simp add: FixedGuardNode.hyps(1))
   have notend: "\<not>(is_AbstractEndNode (kind g nid))"
     by (simp add: FixedGuardNode.hyps(1))
-  from notseq notend 
+  from notseq notend
   show ?case
-    by (smt (verit) IRNode.distinct(373,703,1407,1431,1451,1453,1473,1475,1479) IRNode.inject(13)
-        step.cases Pair_inject FixedGuardNode.hyps(1,5))
+    by (smt (verit) IRNode.distinct(385,1459,1483,1485,1505,1507,1527,1529,1533,1535) step.cases
+        IRNode.inject(13) Pair_inject FixedGuardNode.hyps(1,5) is_preevaluated.simps(8,24))
 next
   case (BytecodeExceptionNode nid args st n' ex h' ref h m' m)
   have notseq: "\<not>(is_sequential_node (kind g nid))"
@@ -138,10 +138,19 @@ next
     by (simp add: BytecodeExceptionNode.hyps(1))
   have notnewarray: "\<not>(is_NewArrayNode (kind g nid))"
     by (simp add: BytecodeExceptionNode.hyps(1))
+  have notarraylength: "\<not>(is_ArrayLengthNode (kind g nid))"
+    by (simp add: BytecodeExceptionNode.hyps(1))
+  have notloadindex: "\<not>(is_LoadIndexedNode (kind g nid))"
+    by (simp add: BytecodeExceptionNode.hyps(1))
+  have notstoreindex: "\<not>(is_StoreIndexedNode (kind g nid))"
+    by (simp add: BytecodeExceptionNode.hyps(1))
   from notseq notif notref notnew notload notstore notdivrem notfixedguard notend notnewarray
+       notarraylength notloadindex notstoreindex
   show ?case
-    by (smt (verit) BytecodeExceptionNode.hyps IRNode.disc(1614,3102) IRNode.inject(7) repDet
-        IRNode.discI(13,15,38) IRNode.distinct(359,751,773,775) Pair_inject step.cases)
+    apply simp
+    by (smt (verit) BytecodeExceptionNode.hyps IRNode.disc(1666,2370,3074,3138,3266) Pair_inject
+        IRNode.inject(7) IRNode.discI(4,53) repDet step.cases notend is_NewInstanceNode_def
+        is_LoadIndexedNode_def is_IntegerDivRemNode.simps is_IfNode_def is_FixedGuardNode_def)
 next
   case (IfNode nid cond tb fb m val "next" h)
   then have notseq: "\<not>(is_sequential_node (kind g nid))"
@@ -155,47 +164,54 @@ next
   from notseq notend notdivrem notnewarray
   show ?case
     by (smt (verit) IRNode.inject(15) Pair_inject repDet evalDet IfNode.hyps step.cases
-        IRNode.distinct(377,707,1407,1613,1633,1635,1655,1657,1661))
+        IRNode.distinct(389,731,1459,1673,1675,1697,1717,1719,1723,1725) IRNode.disc(2370))
 next
   case (EndNodes nid merge i phis inputs m vs m' h)
   have notseq: "\<not>(is_sequential_node (kind g nid))"
-    by (metis is_EndNode.elims(2) is_LoopEndNode_def is_sequential_node.simps(18,35)
+    by (metis is_EndNode.elims(2) is_LoopEndNode_def is_sequential_node.simps(18,36)
         is_AbstractEndNode.simps EndNodes.hyps(1))
   have notif: "\<not>(is_IfNode (kind g nid))"
-    by (metis IRNode.distinct_disc(1620) is_AbstractEndNode.elims(2) EndNodes.hyps(1) is_IfNode_def
+    by (metis IRNode.distinct_disc(1682) is_AbstractEndNode.elims(2) EndNodes.hyps(1) is_IfNode_def
         is_EndNode.simps(16))
   have notref: "\<not>(is_RefNode (kind g nid))"
     by (metis notseq is_RefNode_def is_sequential_node.simps(7))
   have notnew: "\<not>(is_NewInstanceNode (kind g nid))"
-    by (metis IRNode.distinct_disc(2746) is_EndNode.simps(39) is_NewInstanceNode_def
+    by (metis IRNode.distinct_disc(2930) is_EndNode.simps(40) is_NewInstanceNode_def
         is_AbstractEndNode.simps EndNodes.hyps(1))
   have notload: "\<not>(is_LoadFieldNode (kind g nid))"
-    by (metis IRNode.distinct_disc(2544) is_EndNode.simps(28) is_LoadFieldNode_def EndNodes.hyps(1)
+    by (metis IRNode.distinct_disc(2654) is_EndNode.simps(28) is_LoadFieldNode_def EndNodes.hyps(1)
         is_AbstractEndNode.simps)
   have notstore: "\<not>(is_StoreFieldNode (kind g nid))"
-    by (metis IRNode.distinct_disc(2772) is_EndNode.simps(52) is_StoreFieldNode_def EndNodes.hyps(1)
+    by (metis IRNode.distinct_disc(2956) is_EndNode.simps(53) is_StoreFieldNode_def EndNodes.hyps(1)
         is_AbstractEndNode.simps)
   have notdivrem: "\<not>(is_IntegerDivRemNode (kind g nid))"
-    using EndNodes.hyps(1) is_SignedDivNode_def is_SignedRemNode_def by auto
+    using EndNodes.hyps(1) is_SignedDivNode_def is_SignedRemNode_def by force
   have notfixedguard: "\<not>(is_FixedGuardNode (kind g nid))"
-    by (metis IRNode.distinct_disc(1437) is_EndNode.simps(14) is_FixedGuardNode_def EndNodes.hyps(1)
+    by (metis IRNode.distinct_disc(1492) is_EndNode.simps(14) is_FixedGuardNode_def EndNodes.hyps(1)
         is_AbstractEndNode.simps)
   have notbytecodeexception: "\<not>(is_BytecodeExceptionNode (kind g nid))"
-    by (metis IRNode.distinct_disc(738) is_BytecodeExceptionNode_def is_AbstractEndNode.simps
+    by (metis IRNode.distinct_disc(763) is_BytecodeExceptionNode_def is_AbstractEndNode.simps
         is_EndNode.simps(8) EndNodes.hyps(1))
   have notnewarray: "\<not>(is_NewArrayNode (kind g nid))"
-    by (metis IRNode.distinct_disc(2743) is_EndNode.simps(38) is_NewArrayNode_def EndNodes.hyps(1)
+    by (metis IRNode.distinct_disc(2928) is_EndNode.simps(39) is_NewArrayNode_def EndNodes.hyps(1)
         is_AbstractEndNode.simps)
   have notarraylength: "\<not>(is_ArrayLengthNode (kind g nid))"
-    by (metis IRNode.distinct_disc(407) is_EndNode.simps(5) is_ArrayLengthNode_def EndNodes.hyps(1)
+    by (metis IRNode.distinct_disc(421) is_EndNode.simps(5) is_ArrayLengthNode_def EndNodes.hyps(1)
         is_AbstractEndNode.simps)
+  have notloadindex: "\<not>(is_LoadIndexedNode (kind g nid))"
+    by (metis IRNode.distinct_disc(2721) is_EndNode.simps(29) is_LoadIndexedNode_def
+        EndNodes.hyps(1) is_AbstractEndNode.simps)
+  have notstoreindex: "\<not>(is_StoreIndexedNode (kind g nid))"
+    by (metis IRNode.distinct_disc(2957) is_EndNode.simps(54) is_AbstractEndNode.simps
+        EndNodes.hyps(1) is_StoreIndexedNode_def)
   from notseq notif notref notnew notload notstore notdivrem notfixedguard notbytecodeexception
-       notnewarray notarraylength
+       notnewarray notarraylength notloadindex notstoreindex
   show ?case
     by (smt (verit) is_FixedGuardNode_def repAllDet evalAllDet is_IfNode_def EndNodes step.cases
         is_RefNode_def Pair_inject is_LoadFieldNode_def is_NewInstanceNode_def is_StoreFieldNode_def
         is_SignedDivNode_def is_SignedRemNode_def is_IntegerDivRemNode.elims(3) is_NewArrayNode_def
-        is_BytecodeExceptionNode_def is_ArrayLengthNode_def)
+        is_BytecodeExceptionNode_def is_ArrayLengthNode_def is_LoadIndexedNode_def
+        is_StoreIndexedNode_def)
 next
   case (NewArrayNode nid len st n' lenE m length' arrayType h' ref h refNo h'')
   have notseq: "\<not>(is_sequential_node (kind g nid))"
@@ -218,8 +234,8 @@ next
     by (simp add: NewArrayNode.hyps(1))
   from notseq notend notif notload notstore notfixedguard notbytecodeexception notarraylength notnew
   show ?case
-    by (smt (verit) IRNode.discI(27) repDet evalDet Value.inject(2) IRNode.distinct(3131,3129)
-        is_FixedGuardNode_def is_NewInstanceNode_def is_ArrayLengthNode_def is_IfNode_def
+    by (smt (verit) IRNode.disc(1666) repDet Value.inject(2) IRNode.distinct(2735,3327,3329,3335)
+        is_FixedGuardNode_def is_NewInstanceNode_def is_ArrayLengthNode_def is_IfNode_def evalDet
         is_BytecodeExceptionNode_def is_StoreFieldNode_def IRNode.inject EndNodes evalAllDet
         Pair_inject step.cases NewArrayNode)
 next
@@ -240,12 +256,83 @@ next
     by (simp add: ArrayLengthNode.hyps(1))
   have notnewarray: "\<not>(is_NewArrayNode (kind g nid))"
     by (simp add: ArrayLengthNode.hyps(1))
-  from notseq notend notif  notstore notfixedguard notbytecodeexception notnew notnewarray
+  have notloadindex: "\<not>(is_LoadIndexedNode (kind g nid))"
+    by (simp add: ArrayLengthNode.hyps(1))
+  from notseq notend notif notstore notfixedguard notbytecodeexception notnew notnewarray
+       notloadindex
   show ?case
-    by (smt (verit) IRNode.disc(211,221,232,233) Value.inject(2) ArrayLengthNode step.cases evalDet
+    by (smt (verit) IRNode.disc(217,218,239,240,243) Value.inject(2) ArrayLengthNode step.cases
         Pair_inject IRNode.inject is_StoreFieldNode_def is_BytecodeExceptionNode_def is_IfNode_def
         is_ArrayLengthNode_def is_NewInstanceNode_def is_FixedGuardNode_def is_NewArrayNode_def
-        repDet)
+        repDet evalDet)
+next
+  case (LoadIndexedNode nid index gu array nid' indexE m indexVal arrayE ref h arrayVal loaded m')
+  then have notseq: "\<not>(is_sequential_node (kind g nid))"
+    by simp
+  have notend: "\<not>(is_AbstractEndNode (kind g nid))"
+    by (simp add: LoadIndexedNode.hyps(1))
+  have notif: "\<not>(is_IfNode (kind g nid))"
+    by (simp add: LoadIndexedNode.hyps(1))
+  have notref: "\<not>(is_RefNode (kind g nid))"
+    by (simp add: LoadIndexedNode.hyps(1))
+  have notload: "\<not>(is_LoadFieldNode (kind g nid))"
+    by (simp add: LoadIndexedNode.hyps(1))
+  have notstore: "\<not>(is_StoreFieldNode (kind g nid))"
+    by (simp add: LoadIndexedNode.hyps(1))
+  have notdivrem: "\<not>(is_IntegerDivRemNode (kind g nid))"
+    by (simp add: LoadIndexedNode.hyps(1))
+  have notnewarray: "\<not>(is_NewArrayNode (kind g nid))"
+    by (simp add: LoadIndexedNode.hyps(1))
+  have notarraylength: "\<not>(is_ArrayLengthNode (kind g nid))"
+    by (simp add: LoadIndexedNode.hyps(1))
+  have notstoreindex: "\<not>(is_StoreIndexedNode (kind g nid))"
+    by (simp add: LoadIndexedNode.hyps(1))
+  have notfixedguard: "\<not>(is_FixedGuardNode (kind g nid))"
+    by (simp add: LoadIndexedNode.hyps(1))
+  have notbytecodeexception: "\<not>(is_BytecodeExceptionNode (kind g nid))"
+    by (simp add: LoadIndexedNode.hyps(1))
+  have notnew: "\<not>(is_NewInstanceNode (kind g nid))"
+    by (simp add: LoadIndexedNode.hyps(1))
+  from notseq notend notif notref notload notstore notdivrem notnewarray notarraylength notnew
+       notstoreindex notfixedguard notbytecodeexception
+  show ?case
+    by (smt (verit) IRNode.distinct(2757,2759) IRNode.inject(28) Value.inject(2) evalDet repDet
+        LoadIndexedNode.hyps Pair_inject step.cases is_ArrayLengthNode_def is_FixedGuardNode_def
+        is_BytecodeExceptionNode_def is_IfNode_def is_LoadFieldNode_def is_StoreIndexedNode_def
+        is_NewArrayNode_def is_NewInstanceNode_def is_StoreFieldNode_def)
+next
+  case (StoreIndexedNode nid ch val st i gu a nid' indexE m iv arrayE ref valE val0 h av new h' m')
+  then have notseq: "\<not>(is_sequential_node (kind g nid))"
+    by simp
+  have notend: "\<not>(is_AbstractEndNode (kind g nid))"
+    by (simp add: StoreIndexedNode.hyps(1))
+  have notif: "\<not>(is_IfNode (kind g nid))"
+    by (simp add: StoreIndexedNode.hyps(1))
+  have notref: "\<not>(is_RefNode (kind g nid))"
+    by (simp add: StoreIndexedNode.hyps(1))
+  have notload: "\<not>(is_LoadFieldNode (kind g nid))"
+    by (simp add: StoreIndexedNode.hyps(1))
+  have notstore: "\<not>(is_StoreFieldNode (kind g nid))"
+    by (simp add: StoreIndexedNode.hyps(1))
+  have notdivrem: "\<not>(is_IntegerDivRemNode (kind g nid))"
+    by (simp add: StoreIndexedNode.hyps(1))
+  have notnewarray: "\<not>(is_NewArrayNode (kind g nid))"
+    by (simp add: StoreIndexedNode.hyps(1))
+  have notarraylength: "\<not>(is_ArrayLengthNode (kind g nid))"
+    by (simp add: StoreIndexedNode.hyps(1))
+  have notfixedguard: "\<not>(is_FixedGuardNode (kind g nid))"
+    by (simp add: StoreIndexedNode.hyps(1))
+  have notbytecodeexception: "\<not>(is_BytecodeExceptionNode (kind g nid))"
+    by (simp add: StoreIndexedNode.hyps(1))
+  have notnew: "\<not>(is_NewInstanceNode (kind g nid))"
+    by (simp add: StoreIndexedNode.hyps(1))
+  from notseq notend notif notref notload notstore notdivrem notnewarray notarraylength notnew
+       notfixedguard notbytecodeexception
+  show ?case
+    by (smt (verit) IRNode.disc(3305,3326,3327) IRNode.inject(53) StoreIndexedNode.hyps Pair_inject
+        Value.inject(2) is_ArrayLengthNode_def is_IfNode_def is_BytecodeExceptionNode_def evalDet
+        is_FixedGuardNode_def is_LoadFieldNode_def is_NewArrayNode_def step.cases repDet
+        is_StoreIndexedNode_def is_NewInstanceNode_def is_StoreFieldNode_def)
 next
   case (NewInstanceNode nid f obj nxt h' ref h m' m)
   then have notseq: "\<not>(is_sequential_node (kind g nid))"
@@ -268,8 +355,8 @@ next
     by (simp add: NewInstanceNode.hyps(1))
   from notseq notend notif notref notload notstore notdivrem notnewarray notarraylength
   show ?case
-    by (smt (verit) NewInstanceNode step.cases IRNode.disc(1614,2234,3102) IRNode.discI(4,15)
-        Pair_inject IRNode.distinct(753,1453,3173,3175) IRNode.inject(38))
+    by (smt (verit) NewInstanceNode step.cases IRNode.disc(1666,2370,3266) IRNode.discI(4,15)
+        Pair_inject IRNode.distinct(779,1507,2737,3373,3375,3381) IRNode.inject(39))
 next
   case (LoadFieldNode nid f obj nxt m ref h v m')
   then have notseq: "\<not>(is_sequential_node (kind g nid))"
@@ -281,8 +368,28 @@ next
   from notseq notend notdivrem
   show ?case
     by (smt (verit) LoadFieldNode step.cases evalDet IRNode.inject(27) option.discI option.inject
-        IRNode.distinct(401,731,1431,1613,2557,2559,2579,2581,2585) Pair_inject Value.inject(2)
-        repDet)
+        IRNode.distinct(413,755,1483,1673,2647,2667,2669,2689,2691,2695,2697) Pair_inject repDet
+        Value.inject(2))
+next
+  case (SignedDivNode nid x y zero sb nxt m v1 v2 v m' h)
+  then have notseq: "\<not>(is_sequential_node (kind g nid))"
+    by simp
+  have notend: "\<not>(is_AbstractEndNode (kind g nid))"
+    by (simp add: SignedDivNode.hyps(1))
+  from notseq notend
+  show ?case
+    by (smt (verit) IRNode.distinct(457,799,1527,1717,2689,2757,3327,3373,3725,3729,3731) evalDet
+        IRNode.inject(49) step.cases SignedDivNode repDet Pair_inject)
+next
+  case (SignedRemNode nid x y zero sb nxt m v1 v2 v m' h)
+  then have notseq: "\<not>(is_sequential_node (kind g nid))"
+    by simp
+  have notend: "\<not>(is_AbstractEndNode (kind g nid))"
+    by (simp add: SignedRemNode.hyps(1))
+  from notseq notend
+  show ?case
+    by (smt (verit) IRNode.distinct(459,801,1529,1719,2691,2759,3329,3375,3725,3753,3755) evalDet
+        step.cases SignedRemNode repDet Pair_inject IRNode.inject(50))
 next
   case (StaticLoadFieldNode nid f nxt h v m' m)
   then have notseq: "\<not>(is_sequential_node (kind g nid))"
@@ -293,8 +400,8 @@ next
     by (simp add: StaticLoadFieldNode.hyps(1))
   from notseq notend notdivrem
   show ?case
-    by (smt (verit) IRNode.distinct(401,731,1431,1613,2557,2559,2579,2581,2585) IRNode.inject(27)
-        step.cases StaticLoadFieldNode Pair_inject option.distinct(1))
+    by (smt (verit) IRNode.distinct(413,755,1483,1673,2647,2667,2669,2689,2691,2695,2697)
+        IRNode.inject(27) step.cases StaticLoadFieldNode Pair_inject option.distinct(1))
 next
   case (StoreFieldNode nid f newval uu obj nxt m val ref h' h m')
   then have notseq: "\<not>(is_sequential_node (kind g nid))"
@@ -305,9 +412,9 @@ next
     by (simp add: StoreFieldNode.hyps(1))
   from notseq notend notdivrem
   show ?case
-    by (smt (verit) IRNode.distinct(449,779,1479,1661,2585,3135,3179,3509,3531) IRNode.inject(51)
-        step.cases StoreFieldNode evalDet option.discI Pair_inject Value.inject(2) option.inject
-        repDet)
+    by (smt (verit) IRNode.distinct(463,805,1533,1723,2695,2763,3333,3379,3729,3753,3797) evalDet
+        IRNode.inject(52) step.cases StoreFieldNode option.discI Pair_inject Value.inject(2) repDet
+        option.inject)
 next
   case (StaticStoreFieldNode nid f newval uv nxt m val h' h m')
   then have notseq: "\<not>(is_sequential_node (kind g nid))"
@@ -318,29 +425,9 @@ next
     by (simp add: StaticStoreFieldNode.hyps(1))
   from notseq notend notdivrem
   show ?case
-    by (smt (verit) IRNode.distinct(449,779,1479,1661,2585,3135,3179,3509,3531) IRNode.inject(51)
-        step.cases StoreFieldNode StaticStoreFieldNode.hyps option.distinct(1) Pair_inject evalDet
-        repDet)
-next
-  case (SignedDivNode nid x y zero sb nxt m v1 v2 v m' h)
-  then have notseq: "\<not>(is_sequential_node (kind g nid))"
-    by simp
-  have notend: "\<not>(is_AbstractEndNode (kind g nid))"
-    by (simp add: SignedDivNode.hyps(1))
-  from notseq notend
-  show ?case
-    by (smt (verit) IRNode.distinct(443,773,1473,1655,2579,3129,3173,3505,3509) IRNode.inject(48)
-        step.cases SignedDivNode repDet evalDet Pair_inject)
-next
-  case (SignedRemNode nid x y zero sb nxt m v1 v2 v m' h)
-  then have notseq: "\<not>(is_sequential_node (kind g nid))"
-    by simp
-  have notend: "\<not>(is_AbstractEndNode (kind g nid))"
-    by (simp add: SignedRemNode.hyps(1))
-  from notseq notend
-  show ?case
-    by (smt (verit) IRNode.distinct(445,775,1475,1657,2581,3131,3175,3505,3531) IRNode.inject(49)
-        step.cases SignedRemNode repDet evalDet Pair_inject)
+    by (smt (verit) IRNode.distinct(463,805,1533,1723,2695,2763,3333,3379,3729,3753,3797) evalDet
+        IRNode.inject(52) step.cases StoreFieldNode StaticStoreFieldNode.hyps option.distinct(1)
+        Pair_inject repDet)
 qed
 
 lemma stepRefNode:
@@ -369,7 +456,9 @@ lemma step_in_ids:
   assumes "g, p \<turnstile> (nid, m, h) \<rightarrow> (nid', m', h')"
   shows "nid \<in> ids g"
   using assms apply (induct "(nid, m, h)" "(nid', m', h')" rule: step.induct) apply fastforce
-  by (metis IRNode.distinct(465,795,1495,1677,2601,3151,3195,3547,3525,3585) IRNode.disc(1829)
-      is_EndNode.simps(60) is_AbstractEndNode.simps not_in_g)+
+  prefer 4 prefer 14 defer defer
+  using IRNode.distinct(481,823,1551,1741,2713,2781,3351,3397,3747,3771,3813,3831) ids_some
+        apply presburger+
+  by (metis IRNode.disc(1952) is_EndNode.simps(62) is_AbstractEndNode.simps not_in_g)
 
 end
